# Discrete Fast Fourier Transform

Available code files:

* [fft2.sage](https://github.com/darkrenaissance/darkfi/blob/master/script/research/zk/fft/fft2.sage):
  implementation using vandermonde matrices illustrating the theory section below.
* [fft3.sage](https://github.com/darkrenaissance/darkfi/blob/master/script/research/zk/fft/fft3.sage):
  simple example with $n = 4$ showing 3 steps of the algorithm.
* [fft4.sage](https://github.com/darkrenaissance/darkfi/blob/master/script/research/zk/fft/fft4.sage):
  illustrates the full working algorithm.

## Theory

$$ f(x)g(x) âˆˆ ğ”½_{<2n}[x] $$
$$ fg = \sum_{i + j < 2n - 2} a_i b_j x^{i + j} $$
Complexity: $O(n^2)$

Suppose $Ï‰ âˆˆ ğ”½$ is an nth root of unity.

Recall: if $ğ”½ = ğ”½_{p^k}$ then $âˆƒN : ğ”½_{p^N}$
contains all nth roots of unity.

$$ \DFT_Ï‰ : ğ”½^n â†’ ğ”½^n $$
$$ \DFT_Ï‰(f) = (f(Ï‰^0), f(Ï‰^1), â€¦, f(Ï‰^{n - 1})) $$

$$ V_Ï‰ =
\begin{pmatrix}
1 & 1   & 1   & \cdots & 1 \\
1 & Ï‰^1 & Ï‰^2 & \cdots & Ï‰^{n - 1} \\
1 & Ï‰^2 & Ï‰^4 & \cdots & Ï‰^{2(n - 1)} \\
\vdots \\
1 & Ï‰^{n - 1} & Ï‰^{2(n - 1)} & \cdots & Ï‰^{(n - 1)^2} \\
\end{pmatrix}
$$

$$ \DFT_Ï‰(f) = V_Ï‰ Â· f^T $$
since vandermonde multiplication is simply evaluation of a polynomial.

### Lemma: $V_Ï‰^{-1} = \frac{1}{n} V_{Ï‰^{-1}}$

Use $1 + Ï‰ + â‹¯ + Ï‰^{n - 1}$ and compute $V_Ï‰ V_{Ï‰^{-1}}$

Corollary: $\DFT_Ï‰$ is invertible.

### Definitions

1. Convolution $f * g = fg \mod (x^n - 1)$
2. Pointwise product
   $$(a_0, â€¦, a_{n - 1})Â·(b_0, â€¦, b_{n - 1}) =
         (a_0 b_0, â€¦, a_{n - 1} b_{n - 1}) âˆˆ ğ”½^n â†’ ğ”½_{<n}[x]$$

### Theorem: $\DFT_Ï‰(f*g) = \DFT_Ï‰(f)Â·\DFT_Ï‰(g)$

$$ fg = q'(x^n - 1) + f*g  $$
$$ â‡’ f*g = fg + q(x^n - 1) $$
$$ \deg fg â‰¤ 2n - 2        $$

$$
\begin{align}
(f*g)(Ï‰^i) &= f(Ï‰^i)g(Ï‰^i) + q(Ï‰^i)(Ï‰^{in} - 1) \\
           &= f(Ï‰^i)g(Ï‰^i)
\end{align}
$$

### Result

$$ f, g âˆˆ ğ”½_{<n/2}[x] $$
$$ fg = f*g $$
$$ \DFT_Ï‰(f*g) = \DFT_Ï‰(f)Â·\DFT_Ï‰(g) $$
$$ fg = \frac{1}{n} \DFT_{Ï‰^{-1}} (\DFT_Ï‰(f) Â· \DFT_Ï‰(g)) $$

## Finite Field Extension Containing Nth Roots of Unity

$$ Î¼_N = âŸ¨Ï‰âŸ©, |ğ”½_{p^N}^Ã—| = p^N - 1 $$
$$ \textrm{ord}(Ï‰) = n | p^N - 1 $$
but $ğ”½_{p^N}^Ã—$ is cyclic.

For all $d | p^N - 1$, there exists $x âˆˆ ğ”½_{p^N}^Ã—$
with ord$(x) = d$.

Finding $n | p^N - 1$ is sufficient for $Ï‰ âˆˆ ğ”½_{p^N}$
$$ n | p^N - 1 â‡” \textrm{ord}(p) = (â„¤ / nâ„¤)^Ã— $$

## FFT Algorithm Recursive Compute

We recurse to a depth of $\log n$. Since each recursion uses $Ï‰^i$, then
in the final step $Ï‰^i = 1$, and we simply return $f^T$.

We only need to prove a single step of the algorithm produces the desired
result, and then the correctness is inductively proven.

$$
\begin{align}
f(X)    &= a_0 + a_1 X + a_2 X^2 + â‹¯ + a_{n - 1} X^{n - 1} \\
        &= g(X) + X^{n/2} h(X)
\end{align}
$$

### Algorithm

Implementation of this algorithm is available in [fft4.sage](https://github.com/darkrenaissance/darkfi/blob/master/script/research/zk/fft/fft4.sage).
Particularly the function called `calc_dft()`.

**function** DFT($n = 2^d, f(X)$)<br>
<span style="padding-left: 30px;">**if** $n = 1$ **then**</span><br>
<span style="padding-left: 60px;">    **return** $f(X)$</span><br>
<span style="padding-left: 30px;">**end**</span><br>
<span style="padding-left: 30px;">Write $f(X)$ as the sum of two polynomials with equal degree</span><br>
<span style="padding-left: 30px;">$f(X) = g(X) + X^{n/2} h(X)$</span><br>
<span style="padding-left: 30px;">Let $\mathbf{g}, \mathbf{h}$ be the vector representations of $g(X), h(X)$</span><br>
<span style="padding-left: 30px;"></span><br>
<span style="padding-left: 30px;">$\mathbf{r} = \mathbf{g} + \mathbf{h}$</span><br>
<span style="padding-left: 30px;">$\mathbf{s} = (\mathbf{g} - \mathbf{h})Â·(Ï‰^0, â€¦, Ï‰^{n/2 - 1})$</span><br>
<span style="padding-left: 30px;">Let $r(X), s(X)$ be the polynomials represented by the vectors $\mathbf{r}, \mathbf{s}$</span><br>
<span style="padding-left: 30px;"></span><br>
<span style="padding-left: 30px;">Compute $(r(Ï‰^0), â€¦, r(Ï‰^{n/2})) = \textrm{DFT}_{Ï‰^2}(n/2, r(X))$</span><br>
<span style="padding-left: 30px;">Compute $(s(Ï‰^0), â€¦, s(Ï‰^{n/2})) = \textrm{DFT}_{Ï‰^2}(n/2, s(X))$</span><br>
<span style="padding-left: 30px;"></span><br>
<span style="padding-left: 30px;">**return** $(r(Ï‰^0), s(Ï‰^0), r(Ï‰^2), s(Ï‰^2), â€¦, r(Ï‰^{n/2}), s(Ï‰^{n/2}))$</span><br>
end

Sage code:

```python
def calc_dft(Ï‰_powers, f):
    m = len(f)
    if m == 1:
        return f
    g, h = vector(f[:m/2]), vector(f[m/2:])

    r = g + h
    s = dot(g - h, Ï‰_powers)

    Ï‰_powers = vector(Ï‰_i for Ï‰_i in Ï‰_powers[::2])
    rT = calc_dft(Ï‰_powers, r)
    sT = calc_dft(Ï‰_powers, s)

    return list(alternate(rT, sT))
```

### Even Values

$$
\begin{align}
r(X)        &= g(X) + h(X) \\
\\
f(Ï‰^{2i})   &= g(Ï‰^{2i}) + (Ï‰^{2i})^{n/2} h(Ï‰^{2i}) \\
            &= g(Ï‰^{2i}) +                h(Ï‰^{2i}) \\
            &= (g + h)(Ï‰^{2i}) \\
\end{align}
$$

So then we can now compute $DFT_Ï‰(f)_{k=2i} = DFT_{Ï‰^2}(r)$
for the even powers of $f(Ï‰^{2i})$.

### Odd Values

For odd values $k = 2i + 1$

$$
\begin{align}
s(X)        &= (g(X) - h(X))Â·(Ï‰^0, â€¦, Ï‰^{n/2 - 1}) \\
\\
f(X)          &= a_0 + a_1 X + a_2 X^2 + â‹¯ + a_{n - 1} X^{n - 1} \\
              &= g(X) + X^{n/2} h(X) \\
f(Ï‰^{2i + 1}) &= g(Ï‰^{2i + 1}) + (Ï‰^{2i + 1})^{n/2} h(Ï‰^{2i + 1}) \\
\end{align}
$$
But observe that for any $n$th root of unity $Ï‰^n = 1$ and $Ï‰^{n/2} = -1$
$$ (Ï‰^{2i + 1})^{n/2} = Ï‰^{in} Ï‰^{n/2} = Ï‰^{n/2} = -1 $$
$$
\begin{align}
â‡’ f(Ï‰^{2i + 1}) &= g(Ï‰^{2i + 1}) - h(Ï‰^{2i + 1}) \\
                &= (g - h)(Ï‰^{2i + 1})
\end{align}
$$

Let $\mathbf{s} = (\mathbf{g} - \mathbf{h})Â·(Ï‰^0, â€¦, Ï‰^{n/2 - 1})$ be the
representation for $s(X)$. Then we can see that $s(Ï‰^{2i}) = (g - h)(Ï‰^{2i + 1})$
as desired.

So then we can now compute $DFT_Ï‰(f)_{k=2i + 1} = DFT_{Ï‰^2}(s)$
for the odd powers of $f(Ï‰^{2i + 1})$.

## Example

Let $n = 8$
$$
\begin{align}
f(X)    &= (a_0 + a_1 X + a_2 X^2 + a_3 X^3) +     (a_4 X^4 + a_5 X^5 + a_6 X^6 + a_7 X^7) \\
        &= (a_0 + a_1 X + a_2 X^2 + a_3 X^3) + X^4 (a_4     + a_5 X   + a_6 X^2 + a_7 X^3) \\
        &= g(X) + X^{n/2} h(X) \\
g(X)    &=  a_0 + a_1 X + a_2 X^2 + a_3 X^3 \\
h(X)    &=  a_4 + a_5 X + a_6 X^2 + a_7 X^3 \\
\end{align}
$$
Now vectorize $g(X), h(X)$
$$
\begin{align}
\mathbf{g} &= (a_0, a_1, a_2, a_3) \\
\mathbf{h} &= (a_4, a_5, a_6, a_7) \\
\end{align}
$$
Compute reduced polynomials in vector form
$$
\begin{align}
\mathbf{r} &=  \mathbf{g} + \mathbf{h} \\
           &= (a_0 + a_4, a_1 + a_5, a_2 + a_6, a_3 + a_7) \\
\mathbf{s} &= (\mathbf{g} - \mathbf{h})Â·(1, Ï‰, Ï‰^2, Ï‰^3) \\
           &= (a_0 - a_4, a_1 - a_5, a_2 - a_6, a_3 - a_7)Â·(1, Ï‰, Ï‰^2, Ï‰^3) \\
           &= (a_0 - a_4, Ï‰ (a_1 - a_5), Ï‰^2 (a_2 - a_6), Ï‰^3 (a_3 - a_7)) \\
\end{align}
$$
Convert them to polynomials from the vectors. We also expand them out below
for completeness.
$$
\begin{align}
r(X)       &= r_0 + r_1 X + r_2 X^2 + r_3 X^3 \\
           &= (a_0 + a_4) + (a_1 + a_5) X + (a_2 + a_6) X^2 + (a_3 + a_7) X^3 \\
s(X)       &= s_0 + s_1 X + s_2 X^2 + s_3 X^3 \\
           &= (a_0 - a_4) + Ï‰ (a_1 - a_5) X + Ï‰^2 (a_2 - a_6) X^2 + Ï‰^3 (a_3 - a_7) X^3 \\
\end{align}
$$
Compute
$$ \textrm{DFT}_{Ï‰^2}(4, r(X)), \textrm{DFT}_{Ï‰^2}(4, s(X)) $$
The values returned will be
$$
(r(1), s(1), r(Ï‰^2), s(Ï‰^2), r(Ï‰^4), s(Ï‰^4), r(Ï‰^6), s(Ï‰^6))
=
(f(1), f(Ï‰), f(Ï‰^2), f(Ï‰^3), f(Ï‰^4), f(Ï‰^5), f(Ï‰^6), f(Ï‰^7))
$$
Which is the output we return.

### Comparing Evaluations for $f(X)$ and $r(X), s(X)$

We can see the evaluations are correct by substituting in $Ï‰^i$.

We expect that $s(X)$ on the domain $(1, Ï‰^2, Ï‰^4, Ï‰^6)$ produces the values
$(f(1), f(Ï‰^2), f(Ï‰^4), f(Ï‰^6))$, while $r(X)$ on the same domain produces
$(f(Ï‰), f(Ï‰^3), f(Ï‰^5), f(Ï‰^7))$.

#### Even Values

Let $k = 2i$, be an even number. Then note that $k$ is a multiple of 2, so
$4k$ is a multiple of $n â‡’ Ï‰^{4k} = 1$,
$$
\begin{align}
r(X)       &= (a_0 + a_4) + (a_1 + a_5) X + (a_2 + a_6) X^2 + (a_3 + a_7) X^3 \\
r(Ï‰^{2i})  &= (a_0 + a_4) + (a_1 + a_5) Ï‰^{2i} + (a_2 + a_6) Ï‰^{4i} + (a_3 + a_7) Ï‰^{6i} \\
f(Ï‰^k)     &= (a_0 + a_1 Ï‰^k + a_2 Ï‰^{2k} + a_3 Ï‰^{3k}) + Ï‰^{4k} (a_4     + a_5 Ï‰^k   + a_6 Ï‰^{2k} + a_7 Ï‰^{3k}) \\
           &= (a_0 + a_1 Ï‰^k + a_2 Ï‰^{2k} + a_3 Ï‰^{3k}) +        (a_4     + a_5 Ï‰^k   + a_6 Ï‰^{2k} + a_7 Ï‰^{3k}) \\
           &= (a_0 + a_4) + (a_1 + a_5) Ï‰^k + (a_2 + a_6) Ï‰^{2k} + (a_3 + a_7) Ï‰^{3k} \\
           &= f(Ï‰^{2i}) \\
           &= (a_0 + a_4) + (a_1 + a_5) Ï‰^{2i} + (a_2 + a_6) Ï‰^{4i} + (a_3 + a_7) Ï‰^{6i} \\
           &= r(Ï‰^{2i})
\end{align}
$$

#### Odd Values

For $k = 2i + 1$ odd, we have a similar relation where $4k = 8i + 4$, so
$Ï‰^{4k} = Ï‰^4$. But observe that $Ï‰^4 = -1$.
$$
\begin{align}
s(X)       &= (a_0 - a_4) + Ï‰ (a_1 - a_5) X + Ï‰^2 (a_2 - a_6) X^2 + Ï‰^3 (a_3 - a_7) X^3 \\
s(Ï‰^{2i})  &= (a_0 - a_4) + (a_1 - a_5) Ï‰^{2i + 1} + (a_2 - a_6) Ï‰^{4i + 2} + (a_3 - a_7) Ï‰^{6i + 3} \\
f(Ï‰^k)     &= (a_0 + a_1 Ï‰^k + a_2 Ï‰^{2k} + a_3 Ï‰^{3k}) + Ï‰^{4k} (a_4     + a_5 Ï‰^k   + a_6 Ï‰^{2k} + a_7 Ï‰^{3k}) \\
           &= (a_0 + a_1 Ï‰^k + a_2 Ï‰^{2k} + a_3 Ï‰^{3k}) -        (a_4     + a_5 Ï‰^k   + a_6 Ï‰^{2k} + a_7 Ï‰^{3k}) \\
           &= f(Ï‰^{2i + 1}) \\
           &= (a_0 + a_1 Ï‰^{2i + 1} + a_2 Ï‰^{4i + 2} + a_3 Ï‰^{6i + 3}) -  (a_4     + a_5 Ï‰^{2i + 1}   + a_6 Ï‰^{4i + 2} + a_7 Ï‰^{6i + 3}) \\
           &= 
           (a_0  - a_4)
           + (a_1 - a_5) Ï‰^{2i + 1}
           + (a_2 - a_6) Ï‰^{4i + 2}
           + (a_3 - a_7) Ï‰^{6i + 3} \\
           &= s(Ï‰^{2i})
\end{align}
$$

